A bit more starting structure

Imp/Expr/Optimize.lean
@@ -7,14 +7,23 @@ namespace Imp.Expr
 Optimizes an expression by folding constants.
 -/
 def optimize : Expr → Expr
-  | expr => expr
+  | .const i => sorry
+  | .var x => sorry
+  | .un op e => sorry
+  | .bin op e1 e2 => sorry
 
 /--
 Optimization doesn't change the meaning of any expression
 -/
-theorem optimize_ok (e : Expr) : e.eval σ = e.optimize.eval σ := by sorry
+theorem optimize_ok (e : Expr) : e.eval σ = e.optimize.eval σ := by
+  induction e with
+  | const i => sorry
+  | var x => sorry
+  | un op e ih => sorry
+  | bin op e1 e2 ih1 ih2 => sorry
 
 /--
 Optimization doesn't change the meaning of any expression
 -/
-theorem optimize_ok' (e : Expr) : e.eval σ = e.optimize.eval σ := by sorry
+theorem optimize_ok' (e : Expr) : e.eval σ = e.optimize.eval σ := by
+  sorry
