Imp/Stmt/Optimize.lean
@@ -6,4 +6,8 @@ namespace Imp.Stmt
 
 /-- Optimize a statement -/
 def optimize : Stmt → Stmt
-  | stmt => stmt
+  | imp {skip;} => sorry
+  | imp {~s1 ~s2} => sorry
+  | imp {~x := ~e;} => sorry
+  | imp {if (~c) {~s1} else {~s2}} => sorry
+  | imp {while (~c) {~s}} => sorry
